<?xml version="1.0"?>


<!DOCTYPE rdf:RDF [
    <!ENTITY owl "http://www.w3.org/2002/07/owl#" >
    <!ENTITY xsd "http://www.w3.org/2001/XMLSchema#" >
    <!ENTITY rdfs "http://www.w3.org/2000/01/rdf-schema#" >
    <!ENTITY rdf "http://www.w3.org/1999/02/22-rdf-syntax-ns#" >
]>


<rdf:RDF xmlns="http://geographicknowledge.de/vocab/Workflow.rdf#"
     xml:base="http://geographicknowledge.de/vocab/Workflow.rdf"
     xmlns:rdfs="http://www.w3.org/2000/01/rdf-schema#"
     xmlns:owl="http://www.w3.org/2002/07/owl#"
     xmlns:xsd="http://www.w3.org/2001/XMLSchema#"
     xmlns:rdf="http://www.w3.org/1999/02/22-rdf-syntax-ns#">
    <owl:Ontology rdf:about="http://geographicknowledge.de/vocab/Workflow.rdf">
        <rdfs:comment xml:lang="en">Basic workflow ontology for modeling derivation graphs and provenance relations in GIS</rdfs:comment>
        <owl:imports rdf:resource="http://geographicknowledge.de/vocab/AnalysisData.rdf"/>
    </owl:Ontology>
    


    <!-- 
    ///////////////////////////////////////////////////////////////////////////////////////
    //
    // Object Properties
    //
    ///////////////////////////////////////////////////////////////////////////////////////
     -->

    


    <!-- http://geographicknowledge.de/vocab/Workflow.rdf#belongsTo -->

    <owl:ObjectProperty rdf:about="http://geographicknowledge.de/vocab/Workflow.rdf#belongsTo"/>
    


    <!-- http://geographicknowledge.de/vocab/Workflow.rdf#edge -->

    <owl:ObjectProperty rdf:about="http://geographicknowledge.de/vocab/Workflow.rdf#edge">
        <rdfs:comment>A property that links to the (reified) statements of a workflow (workflow edges). Use rdf:subject, rdf:predicate and rdf:object to further link the statement with its elements.</rdfs:comment>
        <rdfs:domain rdf:resource="http://geographicknowledge.de/vocab/Workflow.rdf#Workflow"/>
    </owl:ObjectProperty>
    


    <!-- http://geographicknowledge.de/vocab/Workflow.rdf#edgeOf -->

    <owl:ObjectProperty rdf:about="http://geographicknowledge.de/vocab/Workflow.rdf#edgeOf">
        <owl:inverseOf rdf:resource="http://geographicknowledge.de/vocab/Workflow.rdf#edge"/>
    </owl:ObjectProperty>
    


    <!-- http://geographicknowledge.de/vocab/Workflow.rdf#input -->

    <owl:ObjectProperty rdf:about="http://geographicknowledge.de/vocab/Workflow.rdf#input">
        <rdfs:domain rdf:resource="http://geographicknowledge.de/vocab/Workflow.rdf#Operation"/>
    </owl:ObjectProperty>
    


    <!-- http://geographicknowledge.de/vocab/Workflow.rdf#of -->

    <owl:ObjectProperty rdf:about="http://geographicknowledge.de/vocab/Workflow.rdf#of">
        <rdfs:comment xml:lang="en">An overloaded property for linking resources inside a workflow back with provenance resources</rdfs:comment>
    </owl:ObjectProperty>
    


    <!-- http://geographicknowledge.de/vocab/Workflow.rdf#output -->

    <owl:ObjectProperty rdf:about="http://geographicknowledge.de/vocab/Workflow.rdf#output">
        <rdfs:domain rdf:resource="http://geographicknowledge.de/vocab/Workflow.rdf#Operation"/>
    </owl:ObjectProperty>
    


    <!-- http://geographicknowledge.de/vocab/Workflow.rdf#result -->

    <owl:ObjectProperty rdf:about="http://geographicknowledge.de/vocab/Workflow.rdf#result">
        <rdfs:comment>a property that links to the result of a workflow</rdfs:comment>
        <rdfs:domain rdf:resource="http://geographicknowledge.de/vocab/Workflow.rdf#Workflow"/>
    </owl:ObjectProperty>
    


    <!-- http://geographicknowledge.de/vocab/Workflow.rdf#source -->

    <owl:ObjectProperty rdf:about="http://geographicknowledge.de/vocab/Workflow.rdf#source">
        <rdfs:comment>A property that links to the sources (inputs) of a workflow</rdfs:comment>
        <rdfs:domain rdf:resource="http://geographicknowledge.de/vocab/Workflow.rdf#Workflow"/>
        <rdfs:subPropertyOf rdf:resource="&owl;topObjectProperty"/>
    </owl:ObjectProperty>
    


    <!-- 
    ///////////////////////////////////////////////////////////////////////////////////////
    //
    // Classes
    //
    ///////////////////////////////////////////////////////////////////////////////////////
     -->

    


    <!-- http://geographicknowledge.de/vocab/Workflow.rdf#Operation -->

    <owl:Class rdf:about="http://geographicknowledge.de/vocab/Workflow.rdf#Operation">
        <rdfs:comment xml:lang="en">The event of applying some tool to inputs generating outputs inside a workflow</rdfs:comment>
    </owl:Class>
    


    <!-- http://geographicknowledge.de/vocab/Workflow.rdf#Resource -->

    <owl:Class rdf:about="http://geographicknowledge.de/vocab/Workflow.rdf#Resource">
        <rdfs:comment>Any resource used in a workflow. May be a function or a dataset or data or a reference</rdfs:comment>
    </owl:Class>
    


    <!-- http://geographicknowledge.de/vocab/Workflow.rdf#Workflow -->

    <owl:Class rdf:about="http://geographicknowledge.de/vocab/Workflow.rdf#Workflow">
        <rdfs:comment xml:lang="en">A class for instances that denote workflows. Workflow instances should be connected to triples of the workflow, using RDF reification.</rdfs:comment>
    </owl:Class>
</rdf:RDF>



<!-- Generated by the OWL API (version 3.4.2) http://owlapi.sourceforge.net -->

